added garbage collection and transactions to the BlockCache

disk-betree/BlockCache.dfy
@@ -16,11 +16,17 @@ abstract module BlockInterface {
   datatype Variables<T> = Variables(view: View, reftree: ReferenceTree)
     
   type Lookup = seq<Reference>
+
+  predicate IsLookupStart(k: Constants, s: Variables, ref: Reference)
+  {
+    && ref in s.reftree
+    && !exists ref2 :: ref2 in s.reftree && ref in s.reftree[ref2]
+  }
     
   predicate LookupIsValid(k: Constants, s: Variables, lookup: Lookup)
   {
     && |lookup| > 0
-    && lookup[0] == Root(k)
+    && IsLookupStart(k, s, lookup[0])
     && (forall i :: 0 <= i < |lookup| ==> lookup[i] in s.reftree)
     && (forall i :: 0 <= i < |lookup|-1 ==> lookup[i+1] in s.reftree[lookup[i]])
   }
@@ -37,6 +43,11 @@ abstract module BlockInterface {
   predicate LiveDataAvailable(k: Constants, s: Variables) {
     LiveReferences(k, s) <= s.view.Keys
   }
+
+  predicate OneRoot(k: Constants, s: Variables) {
+    && IsLookupStart(k, s, Root(k))
+    && forall ref :: IsLookupStart(k, s, ref) ==> ref == Root(k)
+  }
   
   function Read<T>(k: Constants, s: Variables, ref: Reference) : T
     requires LiveDataAvailable(k, s)
@@ -45,16 +56,17 @@ abstract module BlockInterface {
     s.view[ref]
   }
     
-  datatype CacheOp<T> =
-    | AllocOp(block: T, successors: iset<Reference>, ref: Reference)
-    | WriteOp(ref: Reference, block: T, successors: iset<Reference>)
-
-  function ApplyToReferenceTree(reftree: ReferenceTree, op: CacheOp) : ReferenceTree {
-    reftree[op.ref := op.successors]
+  predicate Init<T>(k: Constants, s: Variables, block: T) {
+    && s.view == imap[Root(k) := block]
+    && s.reftree == imap[Root(k) := iset{}]
   }
-    
-  function ApplyToView(view: View, op: CacheOp) : View {
-    view[op.ref := op.block]
+
+  predicate Alloc<T>(k: Constants, s: Variables, s': Variables, block: T, successors: iset<Reference>, ref: Reference) {
+    && successors <= LiveReferences(k, s)
+    && ref !in LiveReferences(k, s)
+
+    && s'.reftree == s.reftree[ref := successors]
+    && s'.view == s.view[ref := block]
   }
     
   predicate Write<T>(k: Constants, s: Variables, s': Variables, ref: Reference, block: T, successors: iset<Reference>) {
@@ -64,15 +76,24 @@ abstract module BlockInterface {
     && s'.reftree == s.reftree[ref := successors]
     && s'.view == s.view[ref := block]
   }
-    
-  predicate Alloc<T>(k: Constants, s: Variables, s': Variables, block: T, successors: iset<Reference>, ref: Reference) {
-    && successors <= LiveReferences(k, s)
-    && ref !in LiveReferences(k, s)
 
-    && s'.reftree == s.reftree[ref := successors]
-    && s'.view == s.view[ref := block]
+  predicate IsPath(k: Constants, s: Variables, s': Variables, steps: seq<Step>, path: seq<Variables>)
+    decreases steps, 0
+  {
+    && |path| == |steps| + 1
+    && path[0] == s
+    && Last(path) == s'
+    && (forall i :: 0 <= i < |steps| ==> NextStep(k, path[i], path[i+1], steps[i]))
   }
-    
+  
+  predicate Transaction<T(!new)>(k: Constants, s: Variables, s': Variables, steps: seq<Step>)
+    decreases steps, 1
+  {
+    && 0 < |steps|
+    && (forall i :: 0 <= i < |steps| ==> steps[i].AllocStep? || steps[i].WriteStep?)
+    && (exists path: seq<Variables> :: IsPath(k, s, s', steps, path))
+   }
+  
   predicate GC(k: Constants, s: Variables, s': Variables, ref: Reference) {
     && ref !in LiveReferences(k, s)
     && ref in s.view
@@ -80,20 +101,19 @@ abstract module BlockInterface {
     && s'.reftree == s.reftree
   }
   
-  predicate Init<T>(k: Constants, s: Variables, block: T) {
-    && s.view == imap[Root(k) := block]
-    && s.reftree == imap[Root(k) := iset{}]
-  }
-
   datatype Step<T> =
     | AllocStep(block: T, successors: iset<Reference>, ref: Reference)
     | WriteStep(ref: Reference, block: T, successors: iset<Reference>)
+    | TransactionStep(steps: seq<Step>)
     | GCStep(ref: Reference)
-
-  predicate NextStep(k: Constants, s: Variables, s': Variables, step: Step) {
+    
+  predicate NextStep(k: Constants, s: Variables, s': Variables, step: Step)
+    decreases step
+  {
     match step {
       case AllocStep(block, successors, ref) => Alloc(k, s, s', block, successors, ref)
       case WriteStep(ref, block, successors) => Write(k, s, s', ref, block, successors)
+      case TransactionStep(steps) => Transaction(k, s, s', steps)
       case GCStep(ref) => GC(k, s, s', ref)
     }
   }
@@ -113,6 +133,58 @@ abstract module BlockInterface {
     requires Alloc(k, s, s', block, successors, ref)
     ensures Inv(k, s')
   {
+    forall ref1 | ref1 in LiveReferences(k, s')
+      ensures ref1 in LiveReferences(k, s) + iset{ref}
+    { // OBSERVE?
+    }
   }
   
+  lemma WritePreservesInvariant<T>(k: Constants, s: Variables, s': Variables, ref: Reference, block: T, successors: iset<Reference>)
+    requires Inv(k, s)
+    requires Write(k, s, s', ref, block, successors)
+    ensures Inv(k, s')
+  {
+    forall ref1 | ref1 in LiveReferences(k, s')
+      ensures ref1 in LiveReferences(k, s) + iset{ref}
+    { // OBSERVE?
+    }
+  }
+
+  lemma TransactionPreservesInvariant(k: Constants, s: Variables, s': Variables, steps: seq<Step>)
+    requires Inv(k, s)
+    requires Transaction(k, s, s', steps)
+    ensures Inv(k, s')
+    decreases steps
+  {
+    var path :| IsPath(k, s, s', steps, path);
+    var i := 0;
+    while i < |steps|
+      invariant 0 <= i <= |steps|
+      invariant forall j :: 0 <= j <= i ==> Inv(k, path[j])
+    {
+      NextStepPreservesInvariant(k, path[i], path[i+1], steps[i]);
+      i := i + 1;
+    }
+  }
+
+  lemma GCPreservesInvariant(k: Constants, s: Variables, s': Variables, ref: Reference)
+    requires Inv(k, s)
+    requires GC(k, s, s', ref)
+    ensures Inv(k, s')
+  {
+  }
+
+  lemma NextStepPreservesInvariant(k: Constants, s: Variables, s': Variables, step: Step)
+    requires Inv(k, s)
+    requires NextStep(k, s, s', step)
+    ensures Inv(k, s')
+    decreases step
+  {
+    match step {
+      case AllocStep(block, successors, ref) => AllocPreservesInvariant(k, s, s', block, successors, ref);
+      case WriteStep(ref, block, successors) => WritePreservesInvariant(k, s, s', ref, block, successors);
+      case TransactionStep(steps) => TransactionPreservesInvariant(k, s, s', steps);
+      case GCStep(ref) => GCPreservesInvariant(k, s, s', ref);
+    }
+  }
 }
